working on fixing remove

Dafny/Request.dfy
@@ -2,7 +2,7 @@ include "BloodInventory.dfy"
 include "Alert.dfy"
 datatype request = bloodRequest(bloodType: string, volume: int)
 
-method Request(batchRequest:array<request>, bloodInventory: BloodInventory)
+method Request(batchRequest:array<request>, bloodInventory: BloodInventory) returns(requestResult: array<Blood>)
 requires batchRequest != null
 requires bloodInventory != null
 requires bloodInventory.GetArrayVerification() != null
@@ -10,6 +10,26 @@ requires forall i :: 0 <= i < bloodInventory.GetArrayVerification().Length ==> (
 requires forall i :: 0 <= i < batchRequest.Length ==> (validBloodType(batchRequest[i].bloodType))
 requires bloodInventory.GetArrayVerification().Length < bloodInventory.GetSizeVerificaiton()
 requires forall i :: 0 <= i < batchRequest.Length ==> (batchRequest[i].volume >= bloodInventory.GetBloodCountForBloodTypeVerification(batchRequest[i].bloodType, bloodInventory.GetSizeVerificaiton()))
+ensures bloodInventory == old(bloodInventory)
+ensures forall i :: 0 <= i < batchRequest.Length ==> (batchRequest[i].volume == GetCountOfBloodTypeInArray(requestResult, batchRequest[i].bloodType, requestResult.Length - 1))
 {
+    
+}
 
+function GetCountOfBloodTypeInArray(a: array<Blood>, bloodType: string, indexToCountTo: int): int
+requires a != null
+requires forall i :: 0 <= i < a.Length ==> (a[i] != null)
+reads a
+requires indexToCountTo < a.Length
+requires validBloodType(bloodType)
+{
+    if indexToCountTo < 0
+    then
+        0
+    else
+        if a[indexToCountTo].GetBloodType() == bloodType
+        then
+            1 + GetCountOfBloodTypeInArray(a, bloodType, indexToCountTo - 1)
+        else
+            GetCountOfBloodTypeInArray(a, bloodType, indexToCountTo - 1)
 }
